ll/fmlsext.v
@@ -19,6 +19,7 @@ Definition fmlsext (W : Type) Γ1 Γ2 (fmls : (list W)) := (Γ1 ++ fmls ++ Γ2).
 
 Ltac sfs := simpl ; unfold fmlsext ; simpl.
 Ltac sfseq := simpl ; unfold fmlsext ; simpl ; list_assoc_r' ; reflexivity.
+Ltac sfs_in H := simpl in H ; unfold fmlsext in H ; simpl in H.
 
 Lemma fmlsext_fmlsext: forall V (Γ1 Γ2 Φ1 Φ2 : list V) seq,
   fmlsext Γ1 Γ2 (fmlsext Φ1 Φ2 seq) = fmlsext (Γ1 ++ Φ1) (Φ2 ++ Γ2) seq.
