ll/ll_cam.v
@@ -74,7 +74,7 @@ Definition princ_paramR V A rules prs x xs ys psa psb ca cb rps fpb rsr :=
 Check princ_paramL.  Check princ_paramR.
 
 (* if the cut formula is different from the conclusion of rule(s) prs,
-  then it musts be parametric, not principal *)
+  then it must be parametric, not principal *)
 Lemma princ_paramL_nn_ne' W (A : W) rules dual nl nr any prs 
   drsa drsb psa psb ca cb : rsub prs (fun _ => sing) ->
   fmlsruleg prs psa ca -> 
@@ -111,14 +111,12 @@ Definition princ_paramL_nn_ne W (A : W) rules dual nl nr any prs xs ys
 
 Check princ_paramL_nn_ne.  Check princ_paramL_nn_ne'. 
 
-Lemma princ_paramL_n W (A : W) rules dual n any prs xs ys
-  drsa drsb psa psb ca cb : rsub prs (fun _ => sing) ->
-  fmlsrule xs ys prs psa ca -> leT n (length xs) ->
-  rsub (fmlsruleg prs) rules -> 
-  gen_step2 (osscan dual rules n) A any drsa drsb psa ca psb cb.
-Proof. intros ps lel fpa rsr. 
-eapply gs2_eq.  intro. apply req_sym. apply osscan_eq.
-eapply princ_paramL_nn ; eassumption. Qed.
+Print Implicit gs2_eq.
+
+Definition princ_paramL_n W (A : W) rules dual n any prs xs ys
+  drsa drsb psa psb ca cb rps fa lnx rfr :=
+  gs2_osscann_n (@princ_paramL_nn W (A : W) rules dual n 1 any prs xs ys
+  drsa drsb psa psb ca cb rps fa lnx rfr).
 
 (* note princ_paramL is the case n=1 of this *)
 (* isubfml is generic, not dual due to osscan'_eq *)
@@ -126,9 +124,8 @@ Lemma princ_paramL_n' V (A : LLfml V) rules n any prs x xs ys
   drsa drsb psa psb ca cb : rsub prs (fun _ => sing) ->
   fmlsrule (x :: xs) ys prs psa ca -> rsub (fmlsruleg prs) rules -> 
   gen_step2 (osscan' dual rules n) A any drsa drsb psa ca psb cb.
-Proof. intros ps fpa rsr. 
-eapply gs2_eq.  2: eapply princ_paramL_nn.
-intro. apply req_sym.  apply osscan'_eq.
+Proof. intros ps fpa rsr.  apply gs2_osscann_n'.
+eapply princ_paramL_nn.
 exact ps. exact fpa. simpl. apply leT_n_S. apply leT_0_n.
 exact rsr. Qed.
 
@@ -145,56 +142,6 @@ Definition princ_paramR_n_e V A rules n prs x xs ys
     (@princ_paramL_n' V (dual A)
     rules n empty_relT prs x xs ys drsb drsa psb psa cb ca rps fp rsr))).
 
-(* merge_paramL - dual and isubfml are generic *)
-Lemma merge_paramL' V (A : LLfml V) rules dual any prs x xs ys
-  drsb psa psb ca cb : rsub prs (fun _ => sing) ->
-  merge_ctxt (x :: xs) ys prs psa ca -> rsub (merge_ctxtg prs) rules -> 
-  gen_step2 (osscam dual rules) A any (derrec rules emptyT) drsb psa ca psb cb.
-Proof. intros ps mcp rsmr. unfold gen_step2.
-intros sub fpl fpr dl dr. clear sub fpr.
-clear dl dr. 
-apply osscamI. intros. subst.
-inversion mcp. clear mcp. subst.
-pose (rsubD ps _ c X). simpl in s. destruct s.
-eapply merge_ctns_singleL in H1. cD. subst.
-inversion H3 ; subst ; clear H3. 
-
-(* left premise has cut-formula A *)
-- apply ForallT_2D in fpl. cD. clear fpl fpl1.
-destruct fpl2. simpl in d.
-pose (merge_assoc H6 (merge_sym H10)) as mal. cD.
-pose (merge_assoc H9 (merge_sym H4)) as mar. cD.
-clear H6 H10 H4 H9.
-pose (merge_app mal1 (merge_app (merge_Rnil pl) mar1)).  simpl in m.
-specialize (d _ _ _ eq_refl eq_refl m). clear m mal1 mar1.
-eapply derI. apply (rsubD rsmr).  eapply merge_ctxtgI. 
-apply (merge_ctxtI _ _ _ _ X (merge_sym mal0) (merge_sym mar0)).
-repeat (assumption || apply dlCons || apply dlNil).
-
-(* right premise has cut-formula A *)
-- apply ForallT_2D in fpl. cD. clear fpl2 fpl0.
-destruct fpl1. simpl in d.
-pose (merge_assoc H6 H10) as mal. cD.
-pose (merge_assoc H9 H4) as mar. cD.
-clear H6 H10 H4 H9.
-pose (merge_app mal1 (merge_app (merge_Rnil pr) mar1)).  simpl in m.
-specialize (d _ _ _ eq_refl eq_refl m). clear m mar1 mal1.
-eapply derI. apply (rsubD rsmr). eapply merge_ctxtgI. 
-apply (merge_ctxtI _ _ _ _ X mal0 mar0).
-repeat (assumption || apply dlCons || apply dlNil).
-Qed.
-
-Definition merge_paramL V A rules dual any prs x xs ys :=
-  @merge_paramL' V A rules dual any prs x xs ys (derrec rules emptyT).
-
-(* merge_paramR - specific to dual, isubfml *)
-Definition merge_paramR V A rules prs x xs ys psa psb ca cb rps mcp rsmr :=
-  gs2_osscam_dual' (@merge_paramL _ (dual A : LLfml V)
-  rules dual isubfml prs x xs ys psb psa cb ca rps mcp rsmr).
-
-Check merge_paramL.  Check merge_paramR.
-
-(* this would imply merge_paramL *)
 Lemma merge_paramL_n V (A : LLfml V) rules n any prs x xs ys
   drsb psa psb ca cb : rsub prs (fun _ => sing) ->
   merge_ctxt (x :: xs) ys prs psa ca -> rsub (merge_ctxtg prs) rules -> 
@@ -236,7 +183,28 @@ apply (merge_ctxtI _ _ _ _ X mal0 mar0).
 repeat (assumption || apply dlCons || apply dlNil).
 Qed.
 
+Check merge_paramL_n.
+Print Implicit gs2_osscan'_m.
+
+(* note - could prove this directly, with dual generic, see commit
+  4c29c6c2e2bf82cb755fef961e9c998715b8124b *)
+
+Definition merge_paramL'  V A rules any prs x xs ys drsb psa psb ca cb
+  rps mc rmr := gs2_osscan'_m 
+  (@merge_paramL_n V A rules 1 any prs x xs ys drsb psa psb ca cb rps mc rmr).
+
+Check merge_paramL'.
 Check (fun x => gs2_osscann_n (gs2_osscann_dual' (gs2_osscan'_nn x))).
+
+Definition merge_paramL V A rules (* dual *) any prs x xs ys :=
+  @merge_paramL' V A rules (* dual *) any prs x xs ys (derrec rules emptyT).
+
+(* merge_paramR - specific to dual, isubfml *)
+Definition merge_paramR V A rules prs x xs ys psa psb ca cb rps mcp rsmr :=
+  gs2_osscam_dual' (@merge_paramL _ (dual A : LLfml V)
+  rules (* dual *) isubfml prs x xs ys psb psa cb ca rps mcp rsmr).
+
+Check merge_paramL.  Check merge_paramR.
 
 Definition merge_paramR_n V A rules prs n x xs ys 
     drsa psa psb ca cb rps mcp rsmr :=
@@ -266,9 +234,7 @@ unfold fmlsext in H2. unfold fmlsext in H3.
 simpl in H2. simpl in H3.
 injection H2 as. injection H3 as.
 subst. simpl in H2. injection H2 as. subst.
-simpl in fpl. simpl in fpr.
-unfold fmlsext in fpl. unfold fmlsext in fpr.
-simpl in fpl. simpl in fpr.
+sfs_in fpl. sfs_in fpr.
 inversion fpl. inversion fpr. clear fpl fpr. subst.
 specialize (sub A0 (isub_plusL _ _) _ (fst X) _ (fst X1)).
 destruct sub.  exact (d _ _ _ eq_refl eq_refl H1).  Qed.
@@ -287,9 +253,7 @@ unfold fmlsext in H2. unfold fmlsext in H3.
 simpl in H2. simpl in H3.
 injection H2 as. injection H3 as.
 subst. simpl in H2. injection H2 as. subst.
-simpl in fpl. simpl in fpr.
-unfold fmlsext in fpl. unfold fmlsext in fpr.
-simpl in fpl. simpl in fpr.
+sfs_in fpl. sfs_in fpr.
 inversion fpl. inversion fpr. inversion X2. clear fpl fpr X2. subst.
 specialize (sub B (isub_plusR _ _) _ (fst X) _ (fst X3)).
 destruct sub.  exact (d _ _ _ eq_refl eq_refl H1).  Qed.
@@ -317,8 +281,7 @@ inversion psca. subst. clear psca.
 inversion pscb. subst. clear pscb. 
 inversion X. subst. 
 inversion H0. inversion H. clear X H0 H. subst.
-simpl in fpl. simpl in fpr.
-unfold fmlsext in fpr.  unfold fmlsext in H5.  simpl in fpr.
+simpl in fpl. sfs_in fpr.  unfold fmlsext in H5.
 destruct X0.  simpl in H5. inversion H5. clear H5. subst.
 pose (merge_assoc H1 (merge_sym H3)). cD. clear H1 H3.
 inversion fpl. inversion fpr. subst. cD. clear fpl fpr X2 X3 X4.
@@ -344,8 +307,7 @@ inversion psca. subst. clear psca.
 inversion pscb. subst. clear pscb. 
 apply merge_RnilE in H1.  destruct X. 
 unfold fmlsext in H2.  simpl in H2.  injection H2 as . subst. clear H3.
-simpl in fpl. unfold fmlsext in fpl.  simpl in fpl. 
-inversion fpl. subst. cD. assumption. Qed.
+sfs_in fpl.  inversion fpl. subst. cD. assumption. Qed.
 
 Definition one_bot V A rules ys drsa psa psb ca cb rla rlb :=
   gs2_osscam_dual' (@bot_one V (dual A) rules _ ys drsa psb psa cb ca rlb rla).
@@ -439,7 +401,7 @@ inversion mb as [pso fe]. subst cb.  unfold fmlsext in cae.
 destruct l as [ psa ca ra|psa ca ra|psa ca ra|psa ca ra|psa ca ra|psa ca ra] ; 
 inversion ra ; subst ca ; simpl in cae ; inversion cae ; 
 subst A ; simpl in fe ; inversion fe.
-simpl. unfold fmlsext. simpl.  eapply bot_one.
+sfs.  eapply bot_one.
 eapply OSctxt_eq ; split.  apply Onerule_I.
 - eapply (princ_paramL _ llprinc_sing). 
 apply OSctxt. apply l.  exact (rsub_trans (rsubI _ _ princ_mallI) rs).
@@ -469,8 +431,7 @@ Lemma gs_mall' V (A : LLfml V) rules psa psb ca cb
 Proof. intros ma mb. inversion ma ; subst. destruct X. destruct Φ1.
 destruct mb. destruct f. destruct Φ1.
 - apply gs_osscam_lem.  intros * cae cbe.
-unfold fmlsext in cae.  unfold fmlsext in cbe.
-simpl in cae.  simpl in cbe. 
+sfs_in cae.  sfs_in cbe. 
 destruct l as [ psa ca ra|psa ca ra|psa ca ra|psa ca ra|psa ca ra|psa ca ra] ; 
 destruct l0 as [ psb cb rb|psb cb rb|psb cb rb|psb cb rb|psb cb rb|psb cb rb] ; 
 (* following gets all cases of cut where formulae not duals *)
